Veritas.StateSeqMachine.fsti
@@ -2,6 +2,7 @@ module Veritas.StateSeqMachine
 
 open FStar.Seq
 open Veritas.Record
+open Veritas.SeqAux
 open Veritas.State
 open Veritas.SeqMachine
 
@@ -28,6 +29,22 @@ let ssm_k = SeqMachine StateInit StateFail apply_state_op
 
 (* state seq machine *)
 let ssm = PSM ssm_k key_of
+
+let has_some_put_k (s: seq state_op) =
+  exists_sat_elems Put? s
+
+let last_put_idx_k (s: seq state_op{has_some_put_k s}) =
+  last_index Put? s
+
+let last_put_value_or_null_k (s: seq state_op) =
+  if has_some_put_k s then Put?.v (index s (last_put_idx_k s))
+  else Null
+
+val lemma_first_invalid_implies_invalid_get (s: seq state_op{length s > 0}):
+  Lemma (requires (not (valid ssm_k s) /\ valid ssm_k (prefix s (length s - 1))))
+        (ensures (Get? (index s (length s - 1)) /\
+                  Get?.v (index s (length s - 1)) <> 
+                  last_put_value_or_null_k (prefix s (length s - 1)))) 
 
 (* validity under state seq machine is equivalent to rw_consistency *)
 val lemma_state_sm_equiv_rw_consistent (s: seq state_op):
